---
dg-publish: true
---

$$P_{activa}= I^2_{ef}.R= \left( \frac{V_{R}}{R} \right)^2 R= \frac{V_{R}}{R}$$
$$I_{0}= \frac{Vef}{|Z|}=\frac{V_{0}}{\sqrt{ 2 }|z|}$$. Con $|Z|=\sqrt{ R^2+(X_{L}-X_{C})^2 }$ . Con $X_{L}= \omega L=\frac{V_{L}}{I}$, $X_{C}= \frac{1}{\omega C}= \frac{V_{C}}{I}$.
Cuando el circuito está en resonacia $X_{L}=X_{C}$ con $X_{L}= \omega L$ y  Además, $\omega = 2\pi f$

$farad = \frac{s}{ \Omega}$ 
$$henry= \frac{\Omega}{s}$$
Potencia aparente = potencia reactiva (la que nadie quiere) + pot activa (la que sirve)
$$S=Q+P=V_{ef}.I_{ef}$$
$P = I_{e^f }.V_{ef}.\cos (\varphi_{z})=I^2_{ef}.R$
$Q=I_{ef}.V_{ef}.sen(\varphi_{z})$

$$\varepsilon(t)=V_{0}.\cos(\omega t)=\varepsilon_{0}.\cos(\omega t) $$
Luego $Vef=\frac{V_{0}}{\sqrt{ 2 }}$
